Work in progress on the end of 1

doc/tutorial/code/solutions/ex1a-safe-read-write.fst
@@ -1,6 +1,9 @@
 // BEGIN: ACLs
-module ACLs
+module FileName
   type filename = string
+
+module ACLs
+  open FileName
 
   (* canWrite is a function specifying whether or not a file f can be written *)
   let canWrite (f:filename) = 
@@ -17,32 +20,45 @@ module ACLs
 // BEGIN: SystemIO
 module System.IO
   open ACLs
-  assume val read:   f:filename{canRead f}  -> string
-  assume val write:  f:filename{canWrite f} -> string -> unit
+  open FileName
+  assume val read  : f:filename{canRead f}  -> string
+  assume val write : f:filename{canWrite f} -> string -> unit
 // END: SystemIO
 
 // BEGIN: UntrustedClientCode
 module UntrustedClientCode
-  open ACLs
   open System.IO
+  open FileName
   let passwd  = "C:/etc/password"
   let readme  = "C:/public/README"
   let tmp     = "C:/temp/tempfile"
 // END: UntrustedClientCode
 
-// BEGIN: SafeReadWriteTypes
-  val safeRead : filename -> string
-  val safeWrite : filename -> string -> unit
-// END: SafeReadWriteTypes
-// BEGIN: SafeReadWrite
-  let safeRead f = if ACLs.canRead f then System.IO.read f else "unreadable"
-  let safeWrite f s = if ACLs.canWrite f then System.IO.write f s else ()
-// END: SafeReadWrite
+// BEGIN: StaticChecking
+  let staticChecking () =
+    let v1 = read tmp in
+    let v2 = read readme in
+    (* let v3 = read passwd in -- invalid read, fails type-checking *)
+    write tmp "hello!"
+    (* ; write passwd "junk" -- invalid write , fails type-checking *)
+// END: StaticChecking
 
-  let doitSafe () =
-    let v1 = safeRead tmp in
-    let v2 = safeRead readme in
-    let v3 = safeRead passwd in (* v3 = unreadable *)
-    safeWrite tmp "hello!";
-    safeWrite passwd "junk"; (* contents of passwd are now unaffected *)
-    ()
+// BEGIN: CheckedReadWriteTypes
+  val checkedRead : filename -> string
+  val checkedWrite : filename -> string -> unit
+// END: CheckedReadWriteTypes
+// BEGIN: CheckedReadWrite
+  exception InvalidRead
+  let checkedRead f =
+    if ACLs.canRead f then System.IO.read f else raise InvalidRead
+  exception InvalidWrite
+  let checkedWrite f s =
+    if ACLs.canWrite f then System.IO.write f s else raise InvalidWrite
+// END: CheckedReadWrite
+
+  let dynamicChecking () =
+    let v1 = checkedRead tmp in
+    let v2 = checkedRead readme in
+    let v3 = checkedRead passwd in (* v3 = "unreadable" *)
+    checkedWrite tmp "hello!";
+    checkedWrite passwd "junk" (* contents of passwd are now unaffected *)
